Clean up

new/proof/github_com/goose_lang/goose/testdata/examples/channel_search_replace.v
@@ -1,380 +1,9 @@
-From iris.base_logic.lib Require Import saved_prop ghost_map.
 From New.proof Require Export proof_prelude.
 From New.golang.theory Require Import chan.
 From New.proof.github_com.goose_lang.goose.model.channel
   Require Import chan_au_base simple.
 From New.proof Require Import time sync tok_set.
 From New.generatedproof.github_com.goose_lang.goose.testdata.examples Require Import channel.
-
-From iris_named_props Require Import custom_syntax.
-
-Set Default Proof Using "Type".
-
-Section auth_prop.
-
-Class auth_propG Σ :=
-  {
-    #[local] savedPred_inG :: savedPropG Σ;
-    #[local] gnameSet_inG :: ghost_mapG Σ gname ();
-  }.
-
-Context `{!auth_propG Σ}.
-
-Definition own_aprop_auth γ (P : iProp Σ) (n : nat) : iProp Σ :=
-  ∃ gns,
-    "Hgns" ∷ ghost_map_auth γ 1 (gset_to_gmap () gns) ∗
-    "#Hused" ∷ ([∗ set] γprop ∈ gns, ∃ Q, saved_prop_own γprop DfracDiscarded Q) ∗
-    "#HimpliesP" ∷ □(([∗ set] γprop ∈ gns, ∃ Q, saved_prop_own γprop DfracDiscarded Q ∗ ▷ Q) ∗-∗ ▷ P) ∗
-    "%Hn" ∷ ⌜ size gns = n ⌝.
-#[global] Opaque own_aprop_auth.
-#[local] Transparent own_aprop_auth.
-
-Definition own_aprop_frag γ (P : iProp Σ) (n : nat) : iProp Σ :=
-  ∃ gns,
-    "Hgns" ∷ ([∗ set] γprop ∈ gns, γprop ↪[γ] ()) ∗
-    "#HimpliesP" ∷ □(([∗ set] γprop ∈ gns, ∃ Q, saved_prop_own γprop DfracDiscarded Q ∗ ▷ Q) ∗-∗ ▷ P) ∗
-    "%Hn" ∷ ⌜ size gns = n ⌝.
-#[global] Opaque own_aprop_frag.
-#[local] Transparent own_aprop_frag.
-
-Notation own_aprop γ P := (own_aprop_frag γ P 1).
-
-Lemma own_aprop_auth_alloc :
-  ⊢ |==> ∃ γ, own_aprop_auth γ True 0.
-Proof.
-  iMod (ghost_map_alloc ∅) as (γ) "[H _]".
-  iExists γ. unfold own_aprop_auth. iExists ∅.
-  rewrite gset_to_gmap_empty. iFrame. rewrite !big_sepS_empty //.
-  iModIntro. repeat iSplitL; try done. iModIntro. iIntros "_ "; done.
-Qed.
-
-Lemma own_aprop_auth_add Q γ P n :
-  ⊢ own_aprop_auth γ P n ==∗ own_aprop_auth γ (P ∗ Q) (S n) ∗ own_aprop γ Q.
-Proof.
-  iNamed 1.
-  iMod (saved_prop_alloc Q (DfracOwn 1)) as (γprop) "HQ"; first done.
-  destruct (decide (γprop ∈ gns)).
-  { iDestruct (big_sepS_elem_of_acc _ _ γprop with "Hused") as "[[% Hbad] _]"; first done.
-    iCombine "Hbad HQ" gives "[%Hbad _]". done. }
-  iMod (ghost_map_insert γprop () with "Hgns") as "[Hgns_auth Hgns']".
-  { rewrite lookup_gset_to_gmap_None //. }
-  rewrite -gset_to_gmap_union_singleton.
-  iMod (saved_prop_persist with "HQ") as "#HQ".
-  iModIntro. iSplitR "Hgns'".
-  { iFrame. assert ({[γprop]} ## gns) by set_solver.
-    repeat rewrite !big_sepS_union // !big_sepS_singleton. iFrame "∗#".
-    subst. rewrite size_union // size_singleton /=. iSplitL; last done. iModIntro.
-    iSplit.
-    - iIntros "[HQ' HPs]". iSpecialize ("HimpliesP" with "HPs"). iFrame.
-      iDestruct "HQ'" as (?) "[HQ' HQfact]". iCombine "HQ HQ'" gives "[_ H]".
-      iNext. iRewrite "H". iFrame.
-    - iIntros "[HPfact HQfact]". iSplitR "HPfact HimpliesP".
-      + iExists _; iFrame "#∗".
-      + by iApply "HimpliesP".
-  }
-  iExists {[ _ ]}. rewrite !big_sepS_singleton. iFrame. rewrite size_singleton.
-  iSplitL; last done. iModIntro. iSplit.
-  - iIntros "(% & HQ' & HQfact)". iCombine "HQ HQ'" gives "[_ Heq]".
-    iNext. iRewrite "Heq". iFrame.
-  - iIntros "?". iFrame "#∗".
-Qed.
-
-Lemma own_aprop_auth_reset γ P P' n :
-  ⊢ own_aprop_auth γ P n -∗ own_aprop_frag γ P' n ==∗ own_aprop_auth γ True O.
-Proof.
-  iNamed 1. iNamedSuffix 1 "'".
-  iDestruct (ghost_map_lookup_big with "Hgns [Hgns']") as "%Hsub".
-  { instantiate (1:=gset_to_gmap () gns0). rewrite big_sepM_gset_to_gmap. iFrame. }
-  apply subseteq_dom in Hsub. rewrite !dom_gset_to_gmap in Hsub.
-  apply set_subseteq_size_eq in Hsub as Heq; last lia. subst.
-  iMod (ghost_map_delete_big with "Hgns [Hgns']") as "Hgns".
-  { instantiate (1:=gset_to_gmap () gns). rewrite big_sepM_gset_to_gmap. iFrame. }
-  rewrite map_difference_diag.
-  iModIntro. iExists ∅. rewrite gset_to_gmap_empty. iFrame.
-  rewrite !big_sepS_empty.
-  repeat iSplitL; try done. iModIntro. iIntros "_ "; done.
-Qed.
-
-Lemma own_aprop_frag_0 γ :
-  ⊢ own_aprop_frag γ True 0.
-Proof.
-  iExists ∅. rewrite !big_sepS_empty. repeat iSplitL; try done.
-  iModIntro. by iIntros.
-Qed.
-
-#[global] Instance own_aprop_auth_agree γ P P' n :
-  CombineSepGives (own_aprop_auth γ P n) (own_aprop_frag γ P' n) (▷ P ∗-∗ ▷ P').
-Proof.
-  rewrite /CombineSepGives. iIntros "[@ H]". iNamedSuffix "H" "'".
-  iDestruct (ghost_map_lookup_big with "Hgns [Hgns']") as "%Hsub".
-  { instantiate (1:=gset_to_gmap () gns0). rewrite big_sepM_gset_to_gmap. iFrame. }
-  apply subseteq_dom in Hsub. rewrite !dom_gset_to_gmap in Hsub.
-  apply set_subseteq_size_eq in Hsub as Heq; last lia. subst. clear Hn' Hsub.
-  iModIntro.
-  iSplit.
-  - iIntros "HP". iApply "HimpliesP" in "HP". iApply "HimpliesP'" in "HP". iFrame.
-  - iIntros "HP'". iApply "HimpliesP'" in "HP'". iApply "HimpliesP" in "HP'". iFrame.
-Qed.
-
-#[global] Instance own_aprop_auth_agree' γ P P' n :
-  CombineSepGives (own_aprop_frag γ P' n) (own_aprop_auth γ P n)  (▷ P' ∗-∗ ▷ P).
-Proof.
-  rewrite /CombineSepGives. iIntros "[H H']". iCombine "H' H" gives "[? ?]". iModIntro.
-  iSplit; done.
-Qed.
-
-(* higher cost to prefer [own_aprop_auth_agree]. *)
-#[global] Instance own_aprop_auth_le γ P P' n n' :
-  CombineSepGives (own_aprop_auth γ P n) (own_aprop_frag γ P' n') (⌜ n' ≤ n ⌝)%I | 10.
-Proof.
-  rewrite /CombineSepGives. iIntros "[@ H]". iNamedSuffix "H" "'".
-  iDestruct (ghost_map_lookup_big with "Hgns [Hgns']") as "%Hsub".
-  { instantiate (1:=gset_to_gmap () gns0). rewrite big_sepM_gset_to_gmap. iFrame. }
-  apply subseteq_dom in Hsub. rewrite !dom_gset_to_gmap in Hsub.
-  iModIntro. iPureIntro. apply subseteq_size in Hsub. lia.
-Qed.
-
-#[global] Instance own_aprop_auth_le' γ P P' n n' :
-  CombineSepGives (own_aprop_frag γ P' n') (own_aprop_auth γ P n) (⌜ n' ≤ n ⌝)%I | 10.
-Proof.
-  rewrite /CombineSepGives. iIntros "[H H']". iCombine "H' H" gives %H. iModIntro. done.
-Qed.
-
-#[global] Instance own_aprop_frag_combine γ P P' n n' :
-  CombineSepAs (own_aprop_frag γ P n) (own_aprop_frag γ P' n') (own_aprop_frag γ (P ∗ P') (n + n')).
-Proof.
-  rewrite /CombineSepAs. iIntros "[@ H]". iNamedSuffix "H" "'". rename gns0 into gns'.
-  destruct (decide (gns ∩ gns' = ∅)) as [Hdisj|Hbad].
-  2:{
-    apply set_choose_L in Hbad. destruct Hbad as [γprop Hbad].
-    iDestruct (big_sepS_elem_of_acc _ _ γprop with "Hgns") as "[H1 _]";
-      first set_solver.
-    iDestruct (big_sepS_elem_of_acc _ _ γprop with "Hgns'") as "[H2 _]";
-      first set_solver.
-    iCombine "H1 H2" gives %[Hbad' _]. done.
-  }
-  apply disjoint_intersection_L in Hdisj.
-  iExists (gns ∪ gns'). rewrite big_sepS_union //. iFrame.
-  rewrite big_sepS_union //. rewrite size_union //.
-  iSplitL; last word. iModIntro. iSplit.
-  - iIntros "[H H']". iApply "HimpliesP" in "H". iApply "HimpliesP'" in "H'". iFrame.
-  - iIntros "[H H']". iApply "HimpliesP" in "H". iApply "HimpliesP'" in "H'". iFrame.
-Qed.
-
-End auth_prop.
-#[global] Notation own_aprop γ P := (own_aprop_frag γ P 1).
-
-
-Section waitgroup_idiom.
-
-Class waitgroup_joinG Σ := {
-    #[local] tok_inG :: tok_setG Σ;
-    #[local] auth_inG :: auth_propG Σ;
-  }.
-
-Context `{hG: heapGS Σ, !ffi_semantics _ _}.
-Context `{!globalsGS Σ} {go_ctx : GoContext}.
-Context `{!syncG Σ}.
-Context `{!waitgroup_joinG Σ}.
-
-Record WaitGroup_join_names :=
-  {
-    wg_gn : WaitGroup_names;
-    wg_aprop_gn : gname;
-    wg_not_done_gn : gname;
-  }.
-
-Implicit Types γ : WaitGroup_join_names.
-
-Local Definition wgjN := nroot.@"wgjoin".
-
-(* Internal invariant. Maintains ownership of the waitgroup counter so that
-   Done() can run concurrently to Add. *)
-Local Definition is_wgj_inv wg γ : iProp Σ :=
-  "#His" ∷ is_WaitGroup wg γ.(wg_gn) (wgjN.@"wg") ∗
-  "#Hinv" ∷
-  inv (wgjN.@"inv") (
-      ∃ ctr added done Pdone,
-        "Hwg_ctr" ∷ own_WaitGroup γ.(wg_gn) ctr ∗
-        "Hadded" ∷ own_tok_auth_dfrac γ.(wg_not_done_gn) (DfracOwn (1/2)) added ∗
-        "Hdone_toks" ∷ own_toks γ.(wg_not_done_gn) done ∗
-        "Hdone_aprop" ∷ own_aprop_frag γ.(wg_aprop_gn) Pdone done ∗
-        "Hdone_P" ∷ Pdone ∗
-        "%Hctr_pos" ∷ (⌜ 0 ≤ sint.Z ctr ⌝) ∗
-        "%Hctr" ∷ (⌜ sint.Z ctr = Z.of_nat added - Z.of_nat done ⌝)
-    ).
-
-(** Permission to call `Add`. Calling `Add` will extend `P` with a caller-chosen
-    proposition, as long as `num_added` doesn't overflow. *)
-Definition own_Adder wg (num_added : w32) (P : iProp Σ) : iProp Σ :=
-  ∃ γ P',
-  "Hno_waiters" ∷ own_WaitGroup_waiters γ.(wg_gn) (W32 0) ∗
-  "Haprop" ∷ own_aprop_auth γ.(wg_aprop_gn) P' (sint.nat num_added) ∗
-  "Hadded" ∷ own_tok_auth_dfrac γ.(wg_not_done_gn) (DfracOwn (1/2)) (sint.nat num_added) ∗
-  "%Hadded_pos" ∷ ⌜ 0 ≤ sint.Z num_added ⌝ ∗
-  "HimpliesP" ∷ (P' -∗ P) ∗
-  "#Hinv" ∷ is_wgj_inv wg γ.
-#[global] Opaque own_Adder.
-#[local] Transparent own_Adder.
-
-(** Permission to call `Wait`, knowing that `P` will be true afterwards. *)
-Definition own_Waiter wg (P : iProp Σ) : iProp Σ :=
-  ∃ γ n P',
-  "Hwaiters" ∷ own_WaitGroup_waiters γ.(wg_gn) (W32 1) ∗
-  "Hwait_tok" ∷ own_WaitGroup_wait_token γ.(wg_gn) ∗
-  "Haprop" ∷ own_aprop_auth γ.(wg_aprop_gn) P' n ∗
-  "Hadded" ∷ own_tok_auth_dfrac γ.(wg_not_done_gn) (DfracOwn (1/2)) n ∗
-  "HimpliesP" ∷ (P' -∗ P) ∗
-  "#Hinv" ∷ is_wgj_inv wg γ.
-#[global] Opaque own_Waiter.
-#[local] Transparent own_Waiter.
-
-(** Permission to call `Done` as long as `P` is passed in. *)
-Definition own_Done wg (P : iProp Σ) : iProp Σ :=
-  ∃ γ,
-  "Haprop" ∷ own_aprop γ.(wg_aprop_gn) P ∗
-  "Hdone_tok" ∷ own_toks γ.(wg_not_done_gn) 1 ∗
-  "#Hinv" ∷ is_wgj_inv wg γ.
-#[global] Opaque own_Done.
-#[local] Transparent own_Done.
-
-Lemma waitgroup_join_init wg γwg :
-  is_WaitGroup wg γwg (wgjN.@"wg") ∗
-  own_WaitGroup γwg (W32 0) ∗
-  own_WaitGroup_waiters γwg (W32 0) ={⊤}=∗
-  own_Adder wg (W32 0) True.
-Proof.
-  iIntros "(#His & Hctr_inv & Hwaiters)".
-  iMod own_aprop_auth_alloc as (wg_aprop_gn) "Haprop".
-  iMod own_tok_auth_alloc as (wg_not_done_gn) "[Hadded_inv Hadded]".
-  iExists _. instantiate (1:=ltac:(econstructor)). rewrite /own_Adder /=.
-  iFrame. iSplitR; first word.
-  iMod own_toks_0 as "?". iDestruct own_aprop_frag_0 as "?".
-  iSplitR; first by iIntros "!# ?".
-  iMod (inv_alloc with "[-]") as "$"; last done.
-  iFrame "∗#". word.
-Qed.
-
-Lemma wp_WaitGroup__Add P' wg P num_added :
-  {{{ is_pkg_init sync ∗
-      "Ha" ∷ own_Adder wg num_added P ∗
-      "%Hoverflow" ∷ (⌜ sint.Z num_added < 2^31-1 ⌝)
-  }}}
-    wg @ (ptrT.id sync.WaitGroup.id) @ "Add" #(W64 1)
-  {{{ RET #();
-      own_Adder wg (word.add num_added (W32 1)) (P ∗ P') ∗
-      own_Done wg P'
-  }}}.
-Proof.
-  wp_start_folded as "Hpre". iNamed "Hpre". iNamed "Ha". iNamed "Hinv".
-  wp_apply (wp_WaitGroup__Add with "[$]").
-  iInv "Hinv" as "Hi" "Hclose".
-  iApply fupd_mask_intro; [solve_ndisj|]. iIntros "Hmask". iNext.
-  iNamedSuffix "Hi" "_inv". iExists _; iFrame.
-  iCombine "Hadded Hadded_inv" gives %[_ Heq]. subst.
-  iSplitR; first word.
-  iRight. iFrame.
-  iIntros "Hno_waiters".
-  iIntros "Hwg_ctr_inv". iMod "Hmask" as "_".
-  iMod (own_aprop_auth_add P' with "Haprop") as "[Haprop Hdone_aprop]".
-  iCombine "Hadded Hadded_inv" as "Hadded".
-  iMod (own_tok_auth_S with "Hadded") as "[[Hadded Hadded_inv] Hdone_tok]".
-  iCombineNamed "*_inv" as "Hi".
-  iMod ("Hclose" with "[Hi]").
-  { iNamed "Hi". iFrame. word. }
-  iModIntro. iApply "HΦ". iFrame "∗#".
-  progress replace (S _) with (sint.nat (word.add num_added $ W32 1)) by word.
-  progress replace (sint.nat (word.add _ _)) with (sint.nat num_added + 1)%nat by word.
-  iFrame. iSplitR; first word.
-  iIntros "[? ?]". iFrame. by iApply "HimpliesP".
-Qed.
-
-Lemma wp_WaitGroup__Done P wg :
-  {{{ is_pkg_init sync ∗
-      "Ha" ∷ own_Done wg P ∗
-      "HP" ∷ P
-  }}}
-    wg @ (ptrT.id sync.WaitGroup.id) @ "Done" #()
-  {{{ RET #(); True }}}.
-Proof.
-  wp_start_folded as "Hpre". iNamed "Hpre". iNamed "Ha". iNamed "Hinv".
-  wp_apply (wp_WaitGroup__Done with "[$]").
-  iInv "Hinv" as "Hi" "Hclose".
-  iApply fupd_mask_intro; [solve_ndisj|]. iIntros "Hmask". iNext.
-  iNamedSuffix "Hi" "_inv". iExists _; iFrame.
-  iCombine "Hdone_tok Hdone_toks_inv" as "Hdone_toks_inv". simpl.
-  iCombine "Haprop Hdone_aprop_inv" as "Hdone_aprop_inv".
-  iCombine "Hadded_inv Hdone_toks_inv" gives %Hle.
-  iSplitR; first word. iIntros "Hwg_ctr_inv".
-  iMod "Hmask". iCombineNamed "*_inv" as "Hi". iMod ("Hclose" with "[Hi HP]").
-  { iNamed "Hi". iFrame "Hwg_ctr_inv". iFrame "Hdone_aprop_inv".
-    (* FIXME: iFrame seems to frame [?P] in the goal with whatever prop it sees.. *)
-    iFrame "Hdone_toks_inv". iFrame "Hadded_inv". iFrame. word. }
-  iModIntro. by iApply "HΦ".
-Qed.
-
-Lemma wp_WaitGroup__Wait P wg :
-  {{{ is_pkg_init sync ∗ "Ha" ∷ own_Waiter wg P }}}
-    wg @ (ptrT.id sync.WaitGroup.id) @ "Wait" #()
-  {{{ RET #(); ▷ P ∗ own_Adder wg (W32 0) True }}}.
-Proof.
-  wp_start_folded as "Hpre". iApply wp_fupd. iNamed "Hpre". iNamed "Ha". iNamed "Hinv".
-  wp_apply (wp_WaitGroup__Wait with "[$]").
-  iInv "Hinv" as "Hi" "Hclose".
-  iApply fupd_mask_intro; [solve_ndisj|]. iIntros "Hmask". iNext.
-  iNamedSuffix "Hi" "_inv". iExists _; iFrame. iIntros "%Hctr_zero Hwg_ctr_inv".
-  assert (ctr = W32 0) as -> by word.
-  assert (added = done) as -> by word.
-  iCombine "Hadded Hadded_inv" gives %[_ ->].
-  iCombine "Hdone_aprop_inv Haprop" gives "Heq".
-  iMod (own_aprop_auth_reset with "[$] [$]") as "Haprop".
-  iCombine "Hadded Hadded_inv" as "Hadded".
-  iMod (own_tok_auth_sub done with "[$] [$]") as "[Hadded Hadded_inv]".
-  rewrite Nat.sub_diag. iMod "Hmask" as "_".
-  iRename "Hdone_P_inv" into "Hdone_P".
-  iDestruct own_aprop_frag_0 as "-#Hdone_aprop_inv".
-  iMod own_toks_0 as "Hdone_toks_inv". iCombineNamed "*_inv" as "Hi".
-  iMod ("Hclose" with "[Hi]").
-  { iNamed "Hi". iFrame. word. }
-  iModIntro. iIntros "Hwt".
-  iMod fupd_mask_subseteq as "Hmask"; last iMod (dealloc_wait_token with "[$] [$] [$]") as "H".
-  { solve_ndisj. }
-  { word. }
-  replace (word.sub _ _) with (W32 0) by word.
-  iMod "Hmask" as "_". iModIntro. iApply "HΦ". iFrame.
-  iDestruct "Heq" as "[Heq _]". iFrame "#". iSplitL; last word.
-  iApply "HimpliesP". iApply "Heq". done.
-Qed.
-
-Lemma own_Adder_wand P' wg n P :
-  (P -∗ P') -∗
-  own_Adder wg n P -∗
-  own_Adder wg n P'.
-Proof.
-  iIntros "Hwand". iNamed 1. iFrame "∗#%". iIntros "?".
-  iApply "Hwand". iApply "HimpliesP". done.
-Qed.
-
-Lemma own_Waiter_wand P' wg P :
-  (P -∗ P') -∗
-  own_Waiter wg P -∗
-  own_Waiter wg P'.
-Proof.
-  iIntros "Hwand". iNamed 1. iFrame "∗#%". iIntros "?".
-  iApply "Hwand". iApply "HimpliesP". done.
-Qed.
-
-(* Maybe don't really need a separate own_Waiter? *)
-Lemma start_wait wg n P :
-  own_Adder wg n P ={⊤}=∗ own_Waiter wg P.
-Proof.
-  iNamed 1. iFrame "∗#%". iNamed "Hinv".
-  iMod fupd_mask_subseteq; last iMod (alloc_wait_token with "[$] [$]") as "$"; last done.
-  { solve_ndisj. }
-  { word. }
-Qed.
-
-End waitgroup_idiom.
 
 Section proof.
 Context `{hG: heapGS Σ, !ffi_semantics _ _}.
@@ -404,7 +33,7 @@ Definition search_replace (x y: w64) : list w64 → list w64 :=
 Definition chanP wg (x y: w64) (s: slice.t) : iProp Σ :=
   ∃ (xs: list w64),
     "Hxs" ∷ s ↦* xs ∗
-    "Hwg_done" ∷ own_Done wg (s ↦* (search_replace x y xs)).
+    "Hwg_done" ∷ join.own_Done wg (s ↦* (search_replace x y xs)).
 
 Definition waitgroupN := nroot .@ "waitgroup".
 
@@ -438,7 +67,7 @@ Proof.
   case_bool_decide as Hi.
   (* FIXME: wp_if_destruct doesn't keep the fact around? *)
   - cleanup_bool_decide. wp_pures.
-    wp_auto. wp_apply (wp_WaitGroup__Done with "[$Hwg_done Hxs]").
+    wp_auto. wp_apply (join.wp_WaitGroup__Done with "[$Hwg_done Hxs]").
     { rewrite take_ge; last word. rewrite drop_ge; last word.
       rewrite app_nil_r. iFrame. }
     wp_for_post.
@@ -511,7 +140,7 @@ Proof using chanGhostStateG0 waitgroup_joinG0 syncG0.
   { done. }
   iIntros (ch γch_names) "[#His_chan Hoc]". simpl. wp_auto.
   iMod (init_WaitGroup with "wg") as (?) "H".
-  iMod (waitgroup_join_init with "H") as "Hwg".
+  iMod (join.init with "H") as "Hwg".
   iMod (start_simple_buffered _ _ _ (chanP wg_ptr x y) with "[$His_chan] [$Hoc]") as (γch) "#Hchan".
   iAssert (∃ (i : w64), "i" ∷ i_ptr ↦ i)%I with "[$i]" as "HH".
   wp_for. iNamed "HH". wp_auto.
@@ -527,21 +156,20 @@ Proof using chanGhostStateG0 waitgroup_joinG0 syncG0.
       ∃ (offset : w64) nadded,
         "offset" ∷ offset_ptr ↦ offset ∗
         "Hs" ∷ (slice.slice_f s uint64T offset s.(slice.len_f)) ↦* drop (uint.nat offset) xs ∗
-        "Hwg" ∷ own_Adder wg_ptr nadded
+        "Hwg" ∷ join.own_Adder wg_ptr nadded
           ((slice.slice_f s uint64T 0 offset) ↦* take (uint.nat offset) (search_replace x y xs)) ∗
         "%Hoffset" ∷ ⌜ 0 ≤ sint.Z offset ≤ length xs ⌝ ∗
         "%Hnadded" ∷ ⌜ 0 ≤ workRange * sint.Z nadded ≤ sint.Z offset ∨ sint.nat offset = length xs⌝
     )%I with "[offset Hs Hwg]" as "HH".
   { iFrame. iExists _. rewrite drop_0 take_0.
     erewrite <- slice_slice_trivial. iFrame.
-    iDestruct (own_Adder_wand with "[] Hwg") as "$".
+    iDestruct (join.own_Adder_wand with "[] Hwg") as "$".
     { iIntros "_". iApply own_slice_empty; simpl; word. }
     word. }
   iPersist "s".
   wp_for. iNamed "HH". wp_auto. case_bool_decide.
   { rewrite decide_False // decide_True //. wp_auto.
-    iMod (start_wait with "Hwg") as "Hwg".
-    wp_apply (wp_WaitGroup__Wait with "[$Hwg]").
+    wp_apply (join.wp_WaitGroup__Wait with "[$Hwg]").
     iClear "Hs". iIntros "[Hs Hwg]". subst.
     rewrite take_ge; last len. wp_auto. iApply "HΦ".
     rewrite <- slice_slice_trivial. iFrame. }
@@ -558,7 +186,7 @@ Proof using chanGhostStateG0 waitgroup_joinG0 syncG0.
   iIntros "% [-> H]". iNamed "H". wp_auto.
   wp_pure.
   { unfold nextOffset. word. }
-  wp_auto. wp_apply (wp_WaitGroup__Add with "[$Hwg]").
+  wp_auto. wp_apply (join.wp_WaitGroup__Add with "[$Hwg]").
   { word. }
   iIntros "[Hwg Hdone]".
   wp_auto.
@@ -571,7 +199,7 @@ Proof using chanGhostStateG0 waitgroup_joinG0 syncG0.
   iFrame. iExists _.
   iSplitL "Hs".
   { iApply to_named. iExactEq "Hs". f_equal. f_equal. subst nextOffset. word. }
-  iDestruct (own_Adder_wand with "[] Hwg") as "$".
+  iDestruct (join.own_Adder_wand with "[] Hwg") as "$".
   {
     iIntros "[Hpre Hsuf]".
     iDestruct (own_slice_combine offset with "Hpre Hsuf") as "Hs".
