new/proof/sync_proof/cond.v
@@ -1,4 +1,5 @@
 From New.proof.sync_proof Require Import base mutex.
+Local Existing Instances tokG wg_totalG rw_ghost_varG rw_ghost_wlG rw_ghost_rwmutexG  wg_auth_inG.
 
 Unset Printing Projections.
 
