new/proof/sync_proof/once.v
@@ -4,6 +4,8 @@ From New.proof.sync Require Import atomic.
 
 From iris_named_props Require Import custom_syntax.
 
+Local Existing Instances tokG wg_totalG rw_ghost_varG rw_ghost_wlG rw_ghost_rwmutexG  wg_auth_inG.
+
 (**
 A [sync.Once] will perform exactly one action. The specification realizes this
 by requiring a specification for that action (a pre- and post-condition), a
