new/proof/sync_proof/rwmutex.v
@@ -1,6 +1,6 @@
 From iris.proofmode Require Import environments.
 From New.proof.sync_proof Require Import base mutex sema.
-
+Local Existing Instances tokG wg_totalG rw_ghost_varG rw_ghost_wlG rw_ghost_rwmutexG  wg_auth_inG.
 
 Section proof.
 
