new/proof/sync_proof/waitgroup.v
@@ -1,6 +1,6 @@
 From New.proof.sync_proof Require Import base sema.
 From New.experiments Require Import glob.
-
+Local Existing Instances tokG wg_totalG rw_ghost_varG rw_ghost_wlG rw_ghost_rwmutexG  wg_auth_inG.
 
 Section proof.
 Context `{hG:heapGS Σ, !ffi_semantics _ _}.
